feat: extract constants from addQuot

Lean4Lean/Theory/Quot.lean
@@ -5,12 +5,19 @@ namespace Lean4Lean
 
 open Lean (Name FVarId)
 
+def eqConst := vconst(type_of% @Eq)
+def quotConst := vconst(type_of% @Quot)
+def quotMkConst := vconst(type_of% @Quot.mk)
+def quotIndConst := vconst(type_of% @Quot.ind)
+def quotLiftConst := vconst(type_of% @Quot.lift)
+def quotDefEq := vdefeq(α r β f c a => @Quot.lift α r β f c (Quot.mk r a) ≡ f a)
+
 def VEnv.QuotReady (env : VEnv) : Prop :=
-  env.constants ``Eq = some vconst(type_of% @Eq)
+  env.constants ``Eq = some eqConst
 
 def VEnv.addQuot (env : VEnv) : Option VEnv := do
-  let env ← env.addConst ``Quot vconst(type_of% @Quot)
-  let env ← env.addConst ``Quot.mk vconst(type_of% @Quot.mk)
-  let env ← env.addConst ``Quot.ind vconst(type_of% @Quot.ind)
-  let env ← env.addConst ``Quot.lift vconst(type_of% @Quot.lift)
-  env.addDefEq vdefeq(α r β f c a => @Quot.lift α r β f c (Quot.mk r a) ≡ f a)
+  let env ← env.addConst ``Quot quotConst
+  let env ← env.addConst ``Quot.mk quotMkConst
+  let env ← env.addConst ``Quot.ind quotIndConst
+  let env ← env.addConst ``Quot.lift quotLiftConst
+  env.addDefEq quotDefEq
