Lean4Lean/Theory/Typing/QuotLemmas.lean
@@ -10,9 +10,28 @@ namespace VEnv
 
 theorem addQuot_WF (henv : Ordered env) (hq : QuotReady env) :
     addQuot env = some env' → Ordered env' := by
-  refine with_addConst (cis := [(_, _)]) (hcis := ⟨hq, ⟨⟩⟩) henv
+  refine with_addConst (cis := [.const _ eqConst]) (hcis := ⟨hq, ⟨⟩⟩) henv
     (fun _ => ⟨_, by type_tac⟩) fun henv => ?_
   refine with_addConst henv (fun ⟨quot, _⟩ => ⟨_, by type_tac⟩) fun henv => ?_
   refine with_addConst henv (fun ⟨_, quot, _⟩ => ⟨_, by type_tac⟩) fun henv => ?_
   refine with_addConst henv (fun ⟨_, _, quot, eq, _⟩ => ⟨_, by type_tac⟩) fun henv => ?_
   rintro ⟨_, _, _, _, eq, _⟩ ⟨⟩; exact .defeq henv ⟨by type_tac, by type_tac⟩
+
+section
+variable (henv : addQuot env = some env')
+
+theorem addQuot_objs : env'.HasObjects [.defeq quotDefEq, .const `Quot.lift quotLiftConst,
+    .const `Quot.ind quotIndConst, .const `Quot.mk quotMkConst, .const `Quot quotConst] := by
+  let ⟨env, h, henv⟩ := HasObjects.bind_const (ls := []) trivial henv
+  let ⟨env, h, henv⟩ := HasObjects.bind_const h henv
+  let ⟨env, h, henv⟩ := HasObjects.bind_const h henv
+  obtain ⟨env, h, ⟨⟩⟩ := HasObjects.bind_const h henv
+  exact HasObjects.defeq (df := quotDefEq) h
+
+theorem addQuot_quot : env'.constants ``Quot = quotConst := (addQuot_objs henv).2.2.2.2.1
+theorem addQuot_quotMk : env'.constants ``Quot.mk = quotMkConst := (addQuot_objs henv).2.2.2.1
+theorem addQuot_quotInd : env'.constants ``Quot.ind = quotIndConst := (addQuot_objs henv).2.2.1
+theorem addQuot_quotLift : env'.constants ``Quot.lift = quotLiftConst := (addQuot_objs henv).2.1
+theorem addQuot_defeq : env'.defeqs quotDefEq := (addQuot_objs henv).1
+
+end
